adding JSON support for CACL_Policy

src/CACL.v
@@ -1,6 +1,6 @@
 Require Import Term_Defs Maps ID_Type EqClass.
 
-Require Import Manifest_Set.
+Require Import Manifest_Set JSON JSON_Core.
 
 Require Import List.
 Import ListNotations.
@@ -50,6 +50,100 @@ Global Instance EqClassCACL_Permission `{H : EqClass ID_Type} : EqClass CACL_Per
 
 Definition CACL_Access : Type := (ID_Type * CACL_Permission).
 Definition CACL_Policy : Type := MapC ID_Type (list CACL_Access).
+
+Definition STR_CACL_Access : string := "CACL_Access".
+Definition cacl_read_name_constant : string := "CACL_Read".
+Definition cacl_write_name_constant : string := "CACL_Write".
+Definition cacl_invoke_name_constant : string := "CACL_Invoke".
+
+Definition CACL_Permission_to_JSON (t : CACL_Permission) : JSON := 
+  match t with
+  | CACL_Read => constructor_to_JSON STR_CACL_Access cacl_read_name_constant []
+  | CACL_Write => constructor_to_JSON STR_CACL_Access cacl_write_name_constant []
+  | CACL_Invoke => constructor_to_JSON STR_CACL_Access cacl_invoke_name_constant []
+  end.
+
+Definition CACL_Permission_from_JSON_map : MapC string (JSON -> (ResultT CACL_Permission string)) := 
+  [(cacl_read_name_constant, 
+    constructor_from_JSON STR_CACL_Access (fun _ => resultC CACL_Read));
+    (cacl_write_name_constant, 
+    constructor_from_JSON STR_CACL_Access (fun _ => resultC CACL_Write));
+    (cacl_invoke_name_constant, 
+    constructor_from_JSON STR_CACL_Access (fun _ => resultC CACL_Invoke))].
+
+Definition CACL_Permission_from_JSON (js : JSON) : ResultT CACL_Permission string :=
+  from_JSON_gen STR_CACL_Access CACL_Permission_from_JSON_map js.
+
+Global Instance jsonifiable_CACL_Permission : Jsonifiable CACL_Permission.
+  eapply Build_Jsonifiable with 
+    (to_JSON := CACL_Permission_to_JSON)
+    (from_JSON := CACL_Permission_from_JSON).
+  intuition; simpl in *.
+  
+  unfold CACL_Permission_to_JSON.
+  unfold CACL_Permission_from_JSON.
+  break_match;
+  eapply from_JSON_gen_constructor_to_JSON_works;
+  unfold CACL_Permission_from_JSON_map; try reflexivity.
+Defined.
+
+Global Instance Jsonifiable_CACL_Access `{Jsonifiable ID_Type, Jsonifiable CACL_Permission} : Jsonifiable CACL_Access.
+eapply Build_Jsonifiable with 
+  (to_JSON := pair_to_JSON)
+  (from_JSON := pair_from_JSON).
+simpl_json.
+Defined.
+
+Open Scope string_scope.
+
+Global Instance Stringifiable_CACL_Permission : Stringifiable CACL_Permission :=
+  {
+    to_string := fun b => 
+                  match b with 
+                  | CACL_Read =>   "CACL_Read" 
+                  | CACL_Write =>  "CACL_Write"
+                  | CACL_Invoke => "CACL_Invoke"
+                  end;
+    from_string := fun s => 
+                     match s with
+                     | "CACL_Read" =>   resultC CACL_Read
+                     | "CACL_Write" =>  resultC CACL_Write
+                     | "CACL_Invoke" => resultC CACL_Invoke
+                     | _ => errC "Not a CACL_Access"
+                     end;
+    canonical_stringification := fun b =>
+                                   match b with
+                                   | CACL_Read => eq_refl
+                                   | CACL_Write => eq_refl
+                                   | CACL_Invoke => eq_refl
+                                   end;
+  }.
+
+
+Global Instance Jsonifiable_list_CACL_Access `{Jsonifiable CACL_Permission} : Jsonifiable (list CACL_Access).
+eapply Build_Jsonifiable with 
+(to_JSON := map_serial_to_JSON(* list_CACL_Access_to_JSON *))
+(from_JSON := map_serial_from_JSON (* list_CACL_Access_from_JSON *)).
+intuition; induction a; simpl in *; intuition; eauto;
+repeat (try break_match; simpl in *; subst; eauto; try congruence);
+try rewrite canonical_jsonification in *; 
+try rewrite canonical_stringification in *; 
+repeat find_injection; simpl in *; 
+try find_rewrite; eauto; try congruence.
+Defined.
+
+
+Global Instance Jsonifiable_CACL_Policy `{Stringifiable ID_Type, EqClass ID_Type, Jsonifiable CACL_Permission, Jsonifiable (list CACL_Access)}  : Jsonifiable CACL_Policy.
+eapply Build_Jsonifiable with 
+  (to_JSON := map_serial_to_JSON)
+  (from_JSON := map_serial_from_JSON).
+  intuition; induction a; simpl in *; intuition; eauto;
+  repeat (try break_match; simpl in *; subst; eauto; try congruence);
+  try rewrite canonical_jsonification in *; 
+  try rewrite canonical_stringification in *; 
+  repeat find_injection; simpl in *; 
+  try find_rewrite; eauto; try congruence.
+Defined.
 
 
 Definition eqb_CACL_Access `{H : EqClass ID_Type} (a1 a2 : CACL_Access)  : bool := 
@@ -186,18 +280,6 @@ Definition example_cacl_policy : CACL_Policy :=
      ].
 
 
-(*
-Eval compute  in (CACL_policy_union example_cacl_policy example_cacl_policy).
-*)
-
-Definition test_cacl_compute := (CACL_policy_union example_cacl_policy example_cacl_policy).
-
-
-
-
-
-
-
 Definition CACL_policy_generator_ASP (a:ASP) (p:Plc) : CACL_Policy := 
     match a with 
     | SIG =>   [(p, [(sig_id, CACL_Invoke)])] 
@@ -210,15 +292,23 @@ Definition CACL_policy_generator_ASP (a:ASP) (p:Plc) : CACL_Policy :=
     end.
 
 
-Fixpoint CACL_policy_generator (t:Term) (p:Plc) (pol:CACL_Policy) : CACL_Policy := 
+Fixpoint CACL_policy_generator' (t:Term) (p:Plc) (pol:CACL_Policy) : CACL_Policy := 
     match t with 
     | asp a => CACL_policy_union pol (CACL_policy_generator_ASP a p)
-    | att q t' => (CACL_policy_generator t' q pol)
+    | att q t' => (CACL_policy_generator' t' q pol)
     | lseq t1 t2 => 
-        (CACL_policy_generator t2 p (CACL_policy_generator t1 p pol))
+        (CACL_policy_generator' t2 p (CACL_policy_generator' t1 p pol))
     | bseq _ t1 t2 => 
-        (CACL_policy_generator t2 p (CACL_policy_generator t1 p pol))
+        (CACL_policy_generator' t2 p (CACL_policy_generator' t1 p pol))
     | bpar _ t1 t2 => 
-        (CACL_policy_generator t2 p (CACL_policy_generator t1 p pol))
+        (CACL_policy_generator' t2 p (CACL_policy_generator' t1 p pol))
     end.
+
+Definition CACL_policy_generator (t:Term) (p:Plc) : CACL_Policy := 
+  CACL_policy_generator' t p [].
+
+Definition test_cacl_compute := (CACL_policy_generator certificate_style P0).
+  (* (CACL_policy_union example_cacl_policy example_cacl_policy). *)
+
+Definition test_cacl_compute_json : JSON := to_JSON test_cacl_compute.
 
